

1. Let  $X, Y$  be two random values on  $\mathbb{R}$  and  $\alpha \in \mathbb{R}$  show that

(a)  $\mathbb{E}(\alpha X) = \alpha \mathbb{E}(X)$

(b)  $\mathbb{E}(X + Y) = \mathbb{E}(X) + \mathbb{E}(Y)$

(c) If in addition  $X, Y$  are independent show that

$$V(X + Y) = V(X) + V(Y)$$

**Solution:**

(a) We have that

$$\mathbb{E}(\alpha X) = \int_{\mathbb{R}} \alpha x f_X(x) dx = \alpha \int_{\mathbb{R}} x f_X(x) dx = \alpha \mathbb{E}(X)$$

(b) We have that

$$\begin{aligned} \mathbb{E}(X + Y) &= \int_{\mathbb{R}} \int_{\mathbb{R}} (x + y) f_{X,Y}(x, y) dx dy \\ &= \int_{\mathbb{R}} x \left( \int_{\mathbb{R}} f_{X,Y}(x, y) dy \right) dx + \int_{\mathbb{R}} y \left( \int_{\mathbb{R}} f_{X,Y}(x, y) dx \right) dy \\ &= \int_{\mathbb{R}} x f_X(x) dx + \int_{\mathbb{R}} y f_Y(y) dy \\ &= \mathbb{E}(X) + \mathbb{E}(Y) \end{aligned}$$

Both of the previous equalities are true when  $X, Y$  are random variables taking values on  $\mathbb{R}^n$ .

(c) We have that

$$\begin{aligned} V(X) &= \mathbb{E}(X - \mathbb{E}(X))^2 = \mathbb{E}(X^2 - 2X\mathbb{E}(X) + (\mathbb{E}(X))^2) \\ &= \mathbb{E}(X^2) - \mathbb{E}(2X\mathbb{E}(X)) + (\mathbb{E}(X))^2 \\ &= \mathbb{E}(X^2) - 2(\mathbb{E}(X))^2 + (\mathbb{E}(X))^2 \\ &= \mathbb{E}(X^2) - (\mathbb{E}(X))^2 \end{aligned}$$

we hence have

$$\begin{aligned} V(X + Y) &= \mathbb{E}(X + Y)^2 - (\mathbb{E}(X + Y))^2 \\ &= \mathbb{E}(X^2) + 2\mathbb{E}(XY) + \mathbb{E}(Y^2) - (\mathbb{E}(X))^2 - 2\mathbb{E}(X)\mathbb{E}(Y) + (\mathbb{E}(Y))^2 \\ &= \mathbb{E}(X^2) - (\mathbb{E}(X))^2 + \mathbb{E}(Y^2) - (\mathbb{E}(Y))^2 \\ &\quad + 2\mathbb{E}(XY) - 2\mathbb{E}(X)\mathbb{E}(Y) \end{aligned}$$

Now since  $X, Y$  independent we have that  $\mathbb{E}(XY) = \mathbb{E}(X)\mathbb{E}(Y)$  and hence

$$V(X + Y) = \mathbb{E}(X^2) - (\mathbb{E}(X))^2 + \mathbb{E}(Y^2) - (\mathbb{E}(Y))^2 = V(X) + V(Y)$$

2. Let  $X \sim \mathcal{N}(\mu, \sigma^2)$  show directly using the probability density function that

(a)  $\mathbb{E}(X) = \mu$ ,

(b)  $V(X) = \sigma^2$ .

**Solution:** We now that the probability density function of the one dimensional distribution is given by

$$f_X(x) = \frac{1}{\sqrt{2\pi\sigma^2}} \exp\left(-\frac{(x-\mu)^2}{2\sigma^2}\right).$$

(a) Using the definition of  $\mathbb{E}(X)$  we see that

$$\begin{aligned} \mathbb{E}(X) &= \int_{-\infty}^{\infty} x f_X(x) dx = \int_{-\infty}^{\infty} \frac{x}{\sqrt{2\pi\sigma^2}} \exp\left(-\frac{(x-\mu)^2}{2\sigma^2}\right) dx \\ &= \int_{-\infty}^{\infty} \frac{x-\mu}{\sqrt{2\pi\sigma^2}} \exp\left(-\frac{(x-\mu)^2}{2\sigma^2}\right) dx + \int_{-\infty}^{\infty} \frac{\mu}{\sqrt{2\pi\sigma^2}} \exp\left(-\frac{(x-\mu)^2}{2\sigma^2}\right) dx \\ &= \int_{-\infty}^{\infty} \frac{1}{\sqrt{2\pi\sigma^2}} \left[ -\sigma^2 \exp\left(-\frac{(x-\mu)^2}{2\sigma^2}\right) \right]' dx + \mu \int_{-\infty}^{\infty} \frac{1}{\sqrt{2\pi\sigma^2}} \exp\left(-\frac{(x-\mu)^2}{2\sigma^2}\right) dx \\ &= 0 + \mu \times 1 = \mu \end{aligned}$$

where in the last line we have used the fact  $\lim_{x \rightarrow \pm\infty} \exp\left(-\frac{(x-\mu)^2}{2\sigma^2}\right) = 0$  as well as since  $f_X(x)$  is a probability density function we have that  $\int_{-\infty}^{\infty} f_X(x) dx = 1$

(b) We have that  $V(X) = \mathbb{E}(X - \mathbb{E}(X))^2$  and hence we have

$$V(X) = \int_{-\infty}^{\infty} \frac{(x-\mu)^2}{\sqrt{2\pi\sigma^2}} \exp\left(-\frac{(x-\mu)^2}{2\sigma^2}\right) dx$$

where we have used the fact that  $\mathbb{E}(X) = \mu$  from the first part. We now have

$$\begin{aligned} V(X) &= -\sigma^2 \int_{-\infty}^{+\infty} (x-\mu) \frac{1}{\sqrt{2\pi\sigma^2}} \left[ \exp\left(-\frac{(x-\mu)^2}{2\sigma^2}\right) \right]' dx \\ &= \left[ -\sigma^2 (x-\mu) \frac{1}{\sqrt{2\pi\sigma^2}} \exp\left(-\frac{(x-\mu)^2}{2\sigma^2}\right) \right]_{-\infty}^{\infty} + \sigma^2 \int_{-\infty}^{+\infty} \frac{1}{\sqrt{2\pi\sigma^2}} \exp\left(-\frac{(x-\mu)^2}{2\sigma^2}\right) dx \\ &= 0 + \sigma^2 \times 1 = \sigma^2 \end{aligned}$$